% %@author 张书宁
% %@date 2019-12-02

% \documentclass[12pt]{article}

% \usepackage[top=2cm, bottom=2cm, left=2.5cm, right=2.5cm]{geometry}

% \usepackage{ctex}
% \usepackage{amsmath, amssymb}
% \usepackage{enumerate}

% \begin{document}

% \pagestyle{empty}

\begin{center}
    {\heiti 练习题 1.11}
\end{center}

\begin{enumerate}
    \item % 1
        \begin{enumerate}[(1)]
            \item % 1.1
                1;
            \item % 1.2
                1;
            \item % 1.3
                2;
            \item % 1.4
                $2/3$.
        \end{enumerate}
    \item % 2
        利用等式
        \[
            (n!)^{\frac{1}{n^2}} = \mathrm{e}^{\ln(n!)/n^2}.    
        \]
        令 $a_n = \ln n!$, $b_n = n^2$, 则有
        \[
            \lim_{n\to\infty}\frac{a_{n+1} - a_n}{b_{n+1} - b_n} = \lim_{n\to\infty}\frac{\ln(n+1)! - \ln n!}{(n+1)^2 - n^2} = \lim_{n\to\infty}\frac{\ln(n+1)}{2n+1}.
        \]
        再令 $c_n = \ln(n+1)$, $d_n = 2n+1$, 那么
        \[
            \lim_{n\to\infty}\frac{c_{n+1} - c_n}{b_{n+1} - d_n} = \lim_{n\to\infty}\frac{\ln(n+2) - \ln(n+1)}{2n+3 - (2n + 1)} = \frac12\lim_{n\to\infty}\ln\left(1 + \frac{1}{n+1}\right) = 0.    
        \]
        因此 $\lim\limits_{n\to\infty}(\ln n!)/n^2 = 0$, 即 $\lim\limits_{n\to\infty}(n!)^{1/n^2} = 1$.
    \item % 3
        $4/3$.
    \item % 4
        {\heiti 证明}\quad 令 $x_n = a_1 + 2a_2 + \cdots + na_n$, $y_n = n^2$, 显然 $\{y_n\}$ 是严格递增且趋于 $+\infty$.
        则有
        \begin{align*}
            \lim_{n\to\infty}\frac{x_{n+1} - x_n}{y_{n+1} - y_n} &= \lim_{n\to\infty}\frac{(n+1)a_{n+1}}{(n+1)^2 - n^2} \\
                                                                 &= \lim_{n\to\infty}\frac{(n+1)a_{n+1}}{2n + 1} \\
                                                                 &= \lim_{n\to\infty}\frac{(n+1)a_{n+1}}{2(n+1) - 1} \\
                                                                 &= \lim_{n\to\infty}\frac{a_{n+1}}{2 - \frac{1}{n+1}} \\
                                                                 &= \frac a2.
        \end{align*}
        由 Stolz 定理可得
        \[
            \lim_{n\to\infty}\frac{x_n}{y_n} = \lim_{n\to\infty}\frac{a_1 + 2a_2 + \cdots + na_n}{n^2} = \frac a2.    
        \]
    \item % 5
        设 $a_n = (-1)^{n}$, $b_n = n$, 则有
        \[
            \lim_{n\to\infty}\frac{a_n}{b_n} = \lim_{n\to\infty}\frac{(-1)^n}{n} = 0.    
        \]
        那么
        \[
            \lim_{n\to\infty}\frac{a_{n+1} - a_n}{b_{n+1} - b_n} = \lim_{n\to\infty}\frac{(-1)^{n+1} - (-1)^n}{(n+1) - n} = 2\lim_{n\to\infty}(-1)^{n+1}.    
        \]
        但 $\{(-1)^{n+1}\}$ 的极限是不存在的. 
    \item 6
\end{enumerate}

% \end{document}
