% @author Shuning Zhang
% @date 2019-02-06
\documentclass[a4paper, 11pt]{ctexart}
\usepackage{amsfonts, amsmath, amssymb}
\usepackage{enumerate}
\usepackage[bottom=2cm, left=2.5cm, right=2.5cm, top=2cm]{geometry}
\usepackage{multicol}
\begin{document}
\begin{enumerate}
    \item % 1
    \item % 2
    \item % 3
    \item % 4
        {\heiti 证明}\quad 因为
        \[
            \boldsymbol{x} \in \Bigl(\bigcup_i E_i\Bigr)^c \Rightarrow \boldsymbol{x} \notin \bigcup_i E_i
            \Rightarrow \boldsymbol{x} \notin E_i \Rightarrow \boldsymbol{x} \in E_i^c
            \Rightarrow \boldsymbol{x} \in \bigcap_i E_i^c,    
        \]
        故 $\displaystyle{\Bigl(\bigcup_i E_i\Bigr)^c \subset \bigcap_i E_i^c}$. 反之, 则有 $\displaystyle{\bigcap_i E_i^c \subset \Bigl(\bigcup_i E_i\Bigr)^c}$.
        因此 $\displaystyle{\Bigl(\bigcup_i E_i\Bigr)^c = \bigcap_i E_i^c}$.
        
        同理可得 $\displaystyle{\Bigl(\bigcap_i E_i\Bigr)^c = \bigcup_i E_i^c}$.
    \item % 5
    \item % 6
    \item % 7
    \item % 8
    \item % 9
    \item % 10
    \item % 11
    \item % 12
    \item % 13
\end{enumerate}
\end{document}