% author: Shuning Zhang
% creation date: 2019-12-23
\documentclass[a4paper, 10pt]{ctexart}
\usepackage[top=2cm, bottom=2cm, left=2.5cm, right=2.5cm]{geometry}
\usepackage{enumerate}
\usepackage{amsmath, amssymb}
\begin{document}
\pagestyle{empty}
\begin{enumerate}
    \item % 1
        略.
    \item % 2
    \item % 3
    \item % 4
        {\heiti 证明}\quad 根据题意, 则有
        \[
            \lim_{x\to+\infty}f(x) = \lim_{x\to+\infty}\frac{f(x)\ln x}{\ln x} = \lim_{x\to+\infty}\frac{f'(x)\ln x + f(x)\frac1x}{\frac1x} = \lim_{x\to+\infty}(f(x) + xf'(x)\ln x) = l.    
        \]
    \item % 5
        {\heiti 证明}\quad 一方面, 有
        \begin{align*}
            \lim_{x\to+\infty}f(x) &= \lim_{x\to+\infty}\frac{\mathrm{e}^xf(x)}{\mathrm{e}^x} \\
                                   &= \lim_{x\to+\infty}\frac{\mathrm{e}^xf(x) + \mathrm{e}^xf'(x)}{\mathrm{e}^x} \\
                                   &= \lim_{x\to+\infty}\frac{\mathrm{e}^xf(x) + \mathrm{e}^xf'(x) + \mathrm{e}^xf'(x) + \mathrm{e}^xf''(x)}{\mathrm{e}^x} \\
                                   &= \lim_{x\to+\infty}(f(x) + 2f'(x) + f''(x)) = l.
        \end{align*}
        由此可知 $\lim\limits_{x\to+\infty}(2f'(x) + f''(x)) = 0$. 另一方面, 有
        \begin{align*}
            \lim_{x\to+\infty}f'(x) &= \lim_{x\to+\infty}\frac{\mathrm{e}^{2x}f'(x)}{\mathrm{e}^{2x}} \\
                                    &= \lim_{x\to+\infty}\frac{2\mathrm{e}^{2x}f'(x) + \mathrm{e}^{2x}f''(x)}{2\mathrm{e}^{2x}} \\
                                    &= \lim_{x\to+\infty}\frac{2f'(x) + f''(x)}{2} = 0.
        \end{align*}
        因此 $\lim\limits_{x\to+\infty}f'(x) = 0$, 进一步, 可得出 $\lim\limits_{x\to+\infty}f''(x) = 0$.
\end{enumerate}
\end{document}